Add naive memory verifier and prove read is last write implies consistency

Veritas.Memory.fst
@@ -1,62 +1,294 @@
 module Veritas.Memory
 
 open FStar.BitVector
+open FStar.Classical
 open FStar.Seq
 
 (* address is a 256 bit value *)
 let addr_size = 256
 type addr = bv_t addr_size
 
-(* 
- * Payload of an address is either Null, a special initial value, 
+(*
+ * Payload of an address is either Null, a special initial value,
  * or an integer (TODO: replace integer with something more general)
  *)
-type payload = 
+type payload =
   | Null: payload
   | Value: v:int -> payload
 
-(* Memory: mapping from address to payload *)
-type memory = addr -> payload
-
 (* Memory operation is either a read or a write *)
-type memory_op = 
+type memory_op =
   (* Read operation reading a value v at address a *)
-  | Read: a:addr -> v:payload -> memory_op  
+  | Read: a:addr -> v:payload -> memory_op
   (* Write operation writing a value v at address a *)
   | Write: a:addr -> v:payload -> memory_op
 
 (* Return address of a memory operator *)
-let address_of (o: memory_op): Tot addr = 
+let address_of (o: memory_op): Tot addr =
   match o with
   | Read a _ -> a
   | Write a _ -> a
 
-(* Log is a sequence (list) of memory operations *)
+(* Log is a sequence of memory operations *)
 type memory_op_log = seq memory_op
+
+(* type of an index into a log *)
+type log_index (l:memory_op_log) = i:nat{i < length l}
+
+(* Address of log entry at position i *)
+let address_at_idx (l:memory_op_log) (i:log_index l): Tot addr =
+  address_of (index l i)
+
+(* Is an operation at index i a read op *)
+let is_read_op (l:memory_op_log) (i:log_index l): Tot bool =
+  Read? (index l i)
+
+(* For a read operation, return the read value *)
+let read_value (l:memory_op_log) (i:log_index l{is_read_op l i}): Tot payload =
+  Read?.v (index l i)
+
+(* Is an operation at index i a write op *)
+let is_write_op (l:memory_op_log) (i:log_index l): Tot bool =
+  Write? (index l i)
+
+(* For a write operation, return the written value *)
+let written_value (l:memory_op_log) (i:log_index l{is_write_op l i}): Tot payload =
+  Write?.v (index l i)
+
+(*
+ * Our goal is to define a notion of read-write consistency
+ * for a memory_op_log. We do so using a naive verifier
+ * that materializes the entire memory and checks if every
+ * read operation reads the current value of that address
+ *)
+
+(* Memory: mapping from address to payload *)
+type memory = addr -> payload
+
+(* The state of the naive verifier as it processes the log *)
+noeq type naive_verifier_state =
+  | NFailed: naive_verifier_state
+  | NValid: m:memory -> naive_verifier_state
+
+(* apply function for memory *)
+let apply (m:memory) (o:memory_op{Write? o}): Tot memory =
+  let a = Write?.a o in
+  let v = Write?.v o in
+  fun a' -> if a' = a then v else m a'
+
+(* Naive verifier that verifies read-write consistency of a log given an initial memory *)
+let rec naive_verifier (m:memory) (l:memory_op_log): Tot naive_verifier_state
+  (decreases (length l)) =
+  let n = length l in
+  if n = 0 then NValid m
+  else
+    let l' = slice l 0 (n - 1) in
+    let vs = naive_verifier m l' in
+    if NFailed? vs then NFailed
+    else
+      let o = index l (n - 1) in
+      let m' = NValid?.m vs in
+      if Read? o then
+        if Read?.v o = m' (Read?.a o) then vs else NFailed
+      else
+        NValid (apply m' o)
 
 (* Initial state of memory - all addresses have Null *)
 let init_memory:memory = fun _ -> Null
 
-(* apply function for memory *)
-let apply (m:memory) (o:memory_op): Tot memory = 
-match o with
-  | Read a v -> m
-  | Write a v -> (fun a' -> if a' = a then v else m a') 
-
-(* read-write consistency of a log with respect to an initial state of memory*)
-let rec rw_consistent_helper (m:memory) (l:memory_op_log): Tot bool (decreases (length l)) =
-  let n = length l in
-  if n = 0 then true
-  else 
-    let op = index l 0 in 
-    let l' = slice l 1 n  in 
-    if Read? op 
-    then Read?.v op = m (Read?.a op) && rw_consistent_helper m l'
-    else rw_consistent_helper (apply m op) l'
-
 (*
- * read-write consistency starting from the initial state where all 
+ * read-write consistency starting from the initial state where all
  * addresses are initialized to Null
  *)
-let rw_consistent (l:memory_op_log): Tot bool = rw_consistent_helper init_memory l
+let rw_consistent (l:memory_op_log): Tot bool = NValid? (naive_verifier init_memory l)
+
+(* Identify the last write to an address if it exists *)
+let rec last_write_aux (l:memory_op_log) (a:addr):
+  Tot (option (log_index l))
+  (decreases (length l))
+  =
+  let n = length l in
+  (*
+   * TODO: For some reason, Fstar does not automatically infer that an instance of
+   * option (i:nat{i < n-1}) is also an instance of option (i:nat{i < n}).
+   * This function does this range expansion explicitly by unpacking the option object
+   *)
+  let option_range_expand (o:option (i:nat{i < (n-1)})): Tot (option (i:nat{i < n})) =
+    if None? o then None
+    else Some (Some?.v o)  in
+
+  if n = 0 then None
+  else
+    match index l (n - 1) with
+       | Write a' _ -> if a = a'
+                       then Some (n - 1)
+                       else (
+                         lemma_len_slice l 0 (n - 1);
+                         option_range_expand (last_write_aux (slice l 0 (n - 1)) a)
+                       )
+       | _ -> lemma_len_slice l 0 (n - 1);
+              option_range_expand (last_write_aux (slice l 0 (n - 1)) a)
+
+let rec last_write_is_write_to_a (l:memory_op_log) (a:addr):
+  Lemma (requires (Some? (last_write_aux l a)))
+        (ensures (address_at_idx l (Some?.v (last_write_aux l a)) = a /\
+                  is_write_op l (Some?.v (last_write_aux l a))))
+        (decreases (length l))
+        =
+  let n = length l in
+  if n = 0 then ()
+  else
+    let lastOp = index l (n - 1) in
+    let l' = slice l 0 (n - 1) in
+    match lastOp with
+    | Write a' _ -> if a = a' then ()
+                    else last_write_is_write_to_a l' a
+    | _ -> last_write_is_write_to_a l' a
+
+let rec last_write_is_last_write (l:memory_op_log) (a:addr) (i:log_index l):
+  Lemma (requires (Some? (last_write_aux l a) && i > Some?.v (last_write_aux l a)))
+        (ensures (is_read_op l i || address_at_idx l i <> a))
+        (decreases (length l)) =
+  let n = length l in
+  let wi = Some?.v (last_write_aux l a) in
+  if n = 0 then ()
+  else
+    let lastOp = index l (n - 1) in
+    let l' = slice l 0 (n - 1) in
+    match lastOp with
+    | Write a' _ -> if a = a' then ()
+                    else if i = n - 1 then ()
+                    else last_write_is_last_write l' a i; ()
+    | _ -> if i = n - 1 then ()
+           else last_write_is_last_write l' a i; ()
+
+let rec write_exists_implies_last_write (l:memory_op_log) (i:log_index l):
+  Lemma (requires (is_write_op l i))
+        (ensures (Some? (last_write_aux l (address_at_idx l i))))
+        (decreases (length l)) =
+  let n = length l in
+  let a = address_at_idx l i in
+  if n = 0 then ()
+  else
+    let lastOp = index l (n - 1) in
+    let l' = slice l 0 (n - 1) in
+    if i = n - 1 then ()
+    else
+      write_exists_implies_last_write l' i
+
+let last_write_aux2 (l:memory_op_log) (a:addr):
+  Tot (option (i:(log_index l){address_at_idx l i = a /\ is_write_op l i})) =
+  let optwi = last_write_aux l a in
+  if None? optwi then None
+  else
+    let wi = Some?.v optwi in
+    (last_write_is_write_to_a l a; Some wi)
+
+let last_write (l:memory_op_log) (i:log_index l):
+  Tot (option (j:log_index l{j < i && address_at_idx l j = address_at_idx l i && is_write_op l j})) =
+  let l' = slice l 0 i in
+  let a = address_at_idx l i in
+  let optj = last_write_aux2 l' a in
+  if None? optj then None
+  else
+    let j = Some?.v optj in
+    (
+      lemma_len_slice l 0 i;
+      lemma_index_slice l 0 i j;
+      Some j
+    )
+
+let has_some_write (l:memory_op_log) (a:addr): Tot bool =
+  Some? (last_write_aux2 l a)
+
+let last_write_value (l:memory_op_log) (a:addr{has_some_write l a}): Tot payload =
+  let i = Some?.v (last_write_aux2 l a) in
+  written_value l i
+
+let rec memory_is_last_write (l:memory_op_log) (m:memory) (a:addr):
+  Lemma (requires (has_some_write l a && NValid? (naive_verifier m l)))
+        (ensures (NValid?.m (naive_verifier m l) a = last_write_value l a))
+        (decreases (length l)) =
+  let n = length l in
+  if n = 0 then ()
+  else
+    let l' = (slice l 0 (n - 1)) in
+    if is_write_op l (n- 1) then
+      if a = address_at_idx l (n - 1) then
+        ()
+      else (
+        memory_is_last_write l' m a;
+        lemma_index_slice l 0 (n - 1) (Some?.v (last_write_aux2 l' a))
+      )
+    else (
+      memory_is_last_write l' m a;
+      lemma_index_slice l 0 (n - 1) (Some?.v (last_write_aux2 l' a))
+    )
+
+let rec memory_is_null_without_write (l:memory_op_log) (a:addr):
+  Lemma (requires (has_some_write l a = false /\ NValid? (naive_verifier init_memory l)))
+        (ensures (NValid?.m (naive_verifier init_memory l) a = Null))
+        (decreases (length l)) =
+  let n = length l in
+  if n = 0 then ()
+  else
+    let l' = slice l 0 (n - 1) in
+    if is_write_op l (n - 1) then
+      if address_at_idx l (n - 1) = a then
+        write_exists_implies_last_write l (n - 1)
+      else
+        memory_is_null_without_write l' a
+    else
+      memory_is_null_without_write l' a
+
+let has_prev_write (l:memory_op_log) (i:log_index l): Tot bool =
+  Some? (last_write l i)
+
+let has_no_prev_write (l:memory_op_log) (i:log_index l): Tot bool =
+  None? (last_write l i)
+
+let rec read_last_write_implies_rwconsistent (l:memory_op_log):
+  Lemma (requires (forall (i:log_index l).
+                        is_read_op l i ==>
+                          has_no_prev_write l i && read_value l i = Null ||
+                          has_prev_write l i && read_value l i = written_value l (Some?.v (last_write l i))))
+       (ensures (rw_consistent l))
+       (decreases (length l))
+       =
+  let n = length l in
+  if n = 0 then ()
+  else
+    let l' = slice l 0 (n - 1) in
+    let o = index l (n - 1) in
+    let vs' = naive_verifier init_memory l' in
+    let aux (i:log_index l'):
+      Lemma(is_read_op l' i ==>
+                       has_no_prev_write l' i && read_value l' i = Null ||
+                       has_prev_write l' i && read_value l' i = written_value l' (Some?.v (last_write l' i))) =
+      lemma_index_slice l 0 (n - 1) i;
+      if is_read_op l' i then
+        if has_no_prev_write l' i then
+          // TODO: Do asserts have side-effects? The proof
+          // goes through with the assert, but fails when the assert
+          // is commented out; some kind of forall_intro better here?
+          assert (has_no_prev_write l i)
+        else (
+          assert (has_prev_write l i)
+        )
+      else ()
+      in
+    forall_intro aux; read_last_write_implies_rwconsistent l';
+    assert (NValid? vs');
+    let m' = (NValid?.m vs') in
+    if Write? o then ()
+    else
+      let a = address_of o in
+      if has_some_write l' a then (
+        memory_is_last_write l' init_memory a;
+        assert (is_read_op l (n - 1))
+      )
+      else (
+        memory_is_null_without_write l' a;
+        assert (is_read_op l (n - 1))
+      )
 
